WIP

code/ecdsa/Hacl.Impl.EC.P521.Reduction.fst
@@ -18,7 +18,8 @@ open FStar.Mul
 
 open Hacl.Impl.EC.MontgomeryMultiplication.Lemmas
 
-#set-options " --z3rlimit 200" 
+
+#set-options " --z3rlimit 200 --max_fuel 0 --max_ifuel 0" 
 
 
 let coordinate521 = 9ul
@@ -44,9 +45,13 @@ assume val reduction_prime_2prime:  x: felem-> result: felem ->
       modifies (loc result) h0 h1 /\ lseq_as_nat (as_seq h1 result) == lseq_as_nat (as_seq h0 x) % prime521)
 
 
-#set-options " --z3rlimit 500" 
+val getZeroWord0: a: Lib.Sequence.lseq uint64 8 -> o8: nat -> Lemma ((lseq_as_nat a + (o8 % pow2 9) * pow2 (64 * 8)) < pow2 521)
 
-assume val getZeroWord0: a: Lib.Sequence.lseq uint64 8 -> o8: nat -> Lemma ((lseq_as_nat a + (o8 % pow2 9) * pow2 (64 * 8)) < pow2 521)
+let getZeroWord0 a o8 = 
+  assert((o8 % pow2 9) * pow2 (64 * 8) <= (pow2 9 - 1) * pow2 (64 * 8));
+  lseq_upperbound a;
+  pow2_plus 9 (64 * 8)
+
 
 inline_for_extraction noextract
 val getZeroWord: i: lbuffer uint64 (size 27) -> o: lbuffer uint64 (size 9) -> Stack unit
@@ -56,51 +61,83 @@ val getZeroWord: i: lbuffer uint64 (size 27) -> o: lbuffer uint64 (size 9) -> St
 let getZeroWord i o = 
     let h0 = ST.get() in 
     let iR = sub i (size 0) (size 9) in 
+    
     let iCopy = sub i (size 0) (size 8) in 
     let oCopy = sub o (size 0) (size 8) in 
     let oMaskCopy = sub o (size 8) (size 1) in 
   copy oCopy iCopy;
+
   let o8 = index i (size 8) in 
     let h1 = ST.get() in 
   let o8Updated = logand o8 (u64 0x1ff) in 
   upd o (size 8) o8Updated;
-    assert_norm (pow2 9 - 1 == 0x1ff);
-    logand_mask o8 (u64 0x1ff) 9;
-    let h2 = ST.get() in 
-  lemma_test #9 (as_seq h2 o) 8; 
-  lemma_test (as_seq h1 iR) 8;
-  lseq_as_nat_first (as_seq h2 oMaskCopy);
-  lseq_as_nat_first (Lib.Sequence.sub (as_seq h2 iR) 8 1);
+  let h2 = ST.get() in 
 
-  lemma_test (as_seq h0 i) 9; 
-  pow2_plus (64 * 8 + 9) (64 - 9);
+  let i0 = as_seq h0 i in 
+  let o2 = as_seq h2 o in 
+  let i8 = v (Lib.Sequence.index i0 8) in 
   
+  calc (==) {
+    lseq_as_nat o2;
+  (==) {lemma_test #9 o2 8}
+    (lseq_as_nat (Lib.Sequence.sub o2 0 8) + pow2 (64 * 8) * lseq_as_nat (Lib.Sequence.sub o2 8 1));
+  (==) {lseq_as_nat_first (as_seq h2 oMaskCopy)}
+    (lseq_as_nat (Lib.Sequence.sub (as_seq h0 i) 0 8) + pow2 (64 * 8) * v (Lib.Sequence.index o2 8));
+  (==) {assert_norm (pow2 9 - 1 == 0x1ff); logand_mask o8 (u64 0x1ff) 9}
+    (lseq_as_nat (Lib.Sequence.sub (as_seq h0 i) 0 8) + (v o8 % pow2 9) * pow2 (64 * 8));};
+
+  getZeroWord0 (Lib.Sequence.sub (as_seq h0 i) 0 8) (v o8);
+  small_mod (lseq_as_nat o2) (pow2 521);
+
+
+  calc (==) {lseq_as_nat o2;
+    (==) {}
+  lseq_as_nat o2 % pow2 521;
+    (==) {}
+    (lseq_as_nat (Lib.Sequence.sub (as_seq h0 i) 0 8) + (v o8 % pow2 9) * pow2 (64 * 8)) % pow2 521;
+  (==) {modulo_scale_lemma (v o8) (pow2 (64 * 8)) (pow2 9)}
+    (lseq_as_nat (Lib.Sequence.sub (as_seq h0 i) 0 8) + (v o8 * pow2 (64 * 8) % (pow2 (64 * 8) * pow2 9))) % pow2 521;
+  (==) {pow2_plus (64 * 8) 9}
+    (lseq_as_nat (Lib.Sequence.sub (as_seq h0 i) 0 8) + (i8 * pow2 (64 * 8) % pow2 521)) % pow2 521;
+  (==) {lemma_mod_add_distr (lseq_as_nat (Lib.Sequence.sub (as_seq h0 i) 0 8)) (i8 * pow2 (64 * 8)) (pow2 521)}
+    (lseq_as_nat (Lib.Sequence.sub (as_seq h0 i) 0 8) + i8 * pow2 (64 * 8)) % pow2 521;
+  (==) {lseq_as_nat_first (Lib.Sequence.sub (as_seq h2 iR) 8 1); lemma_test (as_seq h1 iR) 8}
+    lseq_as_nat (as_seq h1 iR) % pow2 521;};
+
+
+  let k =  lseq_as_nat (Lib.Sequence.sub (as_seq h0 i) 9 18) in 
+
   let open FStar.Tactics in 
   let open FStar.Tactics.Canon in 
 
-  assert_by_tactic (pow2 (64 * 8 + 9) * pow2 (64 - 9) * lseq_as_nat (Lib.Sequence.sub (as_seq h0 i) 9 (27 - 9)) ==
-    (pow2 (64 - 9) * lseq_as_nat (Lib.Sequence.sub (as_seq h0 i) 9 (27 - 9))) * pow2 (64 * 8 + 9)) canon;
 
-  modulo_addition_lemma (lseq_as_nat (as_seq h0 iR)) (pow2 (64 * 8 + 9)) (pow2 (64 - 9) * lseq_as_nat (Lib.Sequence.sub (as_seq h0 i) 9 (27 - 9))) ;
+  calc (==) {lseq_as_nat (as_seq h0 i) % pow2 521;
+    (==) {lemma_test (as_seq h0 i) 9}
+  (lseq_as_nat (as_seq h1 iR) + pow2 (521 + 55) * k) % pow2 521;
+    (==) {pow2_plus 521 55}
+  (lseq_as_nat (as_seq h1 iR) + pow2 521 * pow2 55 * k) % pow2 521;
+    (==) {assert_by_tactic (pow2 521 * pow2 55 * k == pow2 521 * (pow2 55 * k)) canon}
+  (lseq_as_nat (as_seq h1 iR) + pow2 521 * (pow2 55 * k)) % pow2 521;  
+    (==) {modulo_addition_lemma (lseq_as_nat (as_seq h1 iR)) (pow2 521) (pow2 55 * k)}
+  (lseq_as_nat (as_seq h1 iR)) % pow2 521;};
 
-  lemma_mod_add_distr (lseq_as_nat (as_seq h0 iCopy)) (pow2 (64 * 8) * v o8) (pow2 521);
 
-  pow2_plus (64 * 8) 9;
-  modulo_scale_lemma (v o8) (pow2 (64 * 8)) (pow2 9);
-  getZeroWord0 (as_seq h0 iCopy) (v o8);
-  small_mod ((lseq_as_nat (as_seq h0 iCopy) + (v o8 % pow2 9) * pow2 (64 * 8))) (pow2 521);
+  assert(lseq_as_nat (as_seq h0 i) % pow2 521 == lseq_as_nat o2)
   
-  assert(lseq_as_nat (as_seq h2 o) == lseq_as_nat (as_seq h0 i) % pow2 521)
+
 
 inline_for_extraction noextract
 val getFirstWord: i: lbuffer uint64 (size 27) -> o: lbuffer uint64 (size 9) -> Stack unit 
-  (requires fun h -> live h i /\ live h o /\ disjoint i o)
+  (requires fun h -> live h i /\ live h o /\ disjoint i o /\ lseq_as_nat (as_seq h o) == 0)
   (ensures fun h0 _ h1 -> modifies (loc o) h0 h1)
 
 let getFirstWord i o = 
   let h0 = ST.get() in 
-  let inv h (j: nat) = live h i /\ live h o /\ modifies (loc o) h0 h in 
+  let inv h (j: nat) = live h i /\ live h o /\ modifies (loc o) h0 h /\ 
+    lseq_as_nat (as_seq h o) == arithmetic_shift_right (lseq_as_nat (as_seq h0 i)) 521 % pow2 (64 * j) in 
+
   Lib.Loops.for 0ul 8ul inv (fun j -> 
+    admit();
     let i0 = index i (size 8 *! size 1 +! j) in 
     let i1 = index i (size 8 *! size 1 +! size 1 +! j) in 
     let i0 = shift_right i0 (size 9) in 
@@ -109,9 +146,15 @@ let getFirstWord i o =
       shift_left_lemma i1 (size 55);
     let o0 = logxor i0 i1U in 
     upd o j o0);
+
+  let h1 = ST.get() in 
+    assert(lseq_as_nat (as_seq h1 o) == arithmetic_shift_right (lseq_as_nat (as_seq h0 i)) 521 % pow2 (64 * 8));
+    
   let o8 = index o (size 8) in 
   let o8Updated = logand o8 (u64 0x1ff) in 
   upd o (size 8) o8Updated
+
+
 
 inline_for_extraction noextract
 val getSecondWord: i: lbuffer uint64 (size 27) -> o: lbuffer uint64 (size 9) -> Stack unit 
